thy/Iptables_Semantics/Common/RepeatStabilize.thy
@@ -2,6 +2,7 @@ theory RepeatStabilize
 imports Main
 begin
 
+section\<open>Repeat finitely Until it Stabilizes\<close>
 text\<open>Repeating something a number of times\<close>
 
 
